WIP

logrel/F_mu.v
@@ -380,7 +380,7 @@ Inductive type :=
 | TProd : type → type → type
 | TSum : type → type → type
 | TArrow : type → type → type
-| TRec : type → type
+| TRec (τ : {bind 1 of type})
 | TVar (x : var)
 | TForall (τ : {bind 1 of type}).
 
@@ -436,10 +436,21 @@ Lemma closed_type_forall {k : nat} {τ : type} :
   closed_type k (TForall τ) → closed_type (S k) τ.
 Proof. intros H; inversion H; subst; trivial. Qed.
 
+Local Hint Resolve closed_type_prod_1 closed_type_prod_2 closed_type_sum_1
+      closed_type_sum_2 closed_type_arrow_1 closed_type_arrow_2
+      closed_type_rec closed_type_var closed_type_forall.
+
 Lemma closed_type_S (k : nat) (τ : type) : closed_type k τ → closed_type (S k) τ.
 Proof. intros H; induction H; auto using closed_type with omega. Qed.
 
 Definition closed_ctx (k : nat) (Γ : list type) := Forall (closed_type k) Γ.
+
+Lemma closed_ctx_S (k : nat) (Γ : list type) : closed_ctx k Γ → closed_ctx (S k) Γ.
+Proof. intros H. eapply Forall_impl; [| apply closed_type_S]; trivial. Qed.
+
+Lemma closed_ctx_closed_type (k : nat) (Γ : list type) (x : var) (τ : type) :
+  closed_ctx k Γ → Γ !! x = Some τ → closed_type k τ.
+Proof. intros; eapply Forall_lookup; eauto. Qed.
 
 Program Fixpoint zipwith_Forall {A : Type} {P : A → Prop} (l : list A) (H : Forall P l) :
   list ({x : A | P x}) :=
@@ -462,13 +473,13 @@ Definition closed_ctx_list (k : nat) (Γ : list type) (H : closed_ctx k Γ) :
 
 Inductive typed (k : nat) (Γ : list type) : expr → type → Prop :=
 | Var_typed x τ : (closed_ctx k Γ) → Γ !! x = Some τ → typed k Γ (Var x) τ
-| Unit_typed : typed k Γ Unit TUnit
+| Unit_typed : closed_ctx k Γ → typed k Γ Unit TUnit
 | Pair_typed e1 e2 τ1 τ2 :
     typed k Γ e1 τ1 → typed k Γ e2 τ2 → typed k Γ (Pair e1 e2) (TProd τ1 τ2)
 | Fst_typed e τ1 τ2 : typed k Γ e (TProd τ1 τ2) → typed k Γ (Fst e) τ1
 | Snd_typed e τ1 τ2 : typed k Γ e (TProd τ1 τ2) → typed k Γ (Snd e) τ2
-| InjL_typed e τ1 τ2 : typed k Γ e τ1 → typed k Γ (InjL e) (TSum τ1 τ2)
-| InjR_typed e τ1 τ2 : typed k Γ e τ2 → typed k Γ (InjR e) (TSum τ1 τ2)
+| InjL_typed e τ1 τ2 : typed k Γ e τ1 → closed_type k τ2 → typed k Γ (InjL e) (TSum τ1 τ2)
+| InjR_typed e τ1 τ2 : typed k Γ e τ2 → closed_type k τ1 → typed k Γ (InjR e) (TSum τ1 τ2)
 | Case_typed e0 e1 e2 τ1 τ2 ρ :
     typed k Γ e0 (TSum τ1 τ2) →
     typed k (τ1 :: Γ) e1 ρ → typed k (τ2 :: Γ) e2 ρ →
@@ -481,13 +492,168 @@ Inductive typed (k : nat) (Γ : list type) : expr → type → Prop :=
     typed (S k) (map (λ t, t.[ren (lift 1)]) Γ) e τ →
     typed k Γ (TLam e) (TForall τ)
 | TApp_typed e τ τ':
-    typed k Γ e (TForall τ) → closed_type k τ' → typed k Γ (TApp e) (τ.[τ'/])
+    typed k Γ e (TForall τ) → closed_type k τ' → typed k Γ (TApp e) (τ.[τ' .: (ren pred)])
 | TFold e τ :
     typed (S k) (map (λ t, t.[ren (lift 1)]) Γ) e τ →
     typed k Γ (Fold e) (TRec τ)
-| TUnfold e τ : typed k Γ e (TRec τ) → typed k Γ (Unfold e) (τ.[(TRec τ)/])
+| TUnfold e τ : typed k Γ e (TRec τ) → typed k Γ (Unfold e) (τ.[(TRec τ) .: (ren pred)])
 .
 
+Lemma closed_type_subst_invariant k τ s1 s2 :
+  closed_type k τ → (∀ x, x < k → s1 x = s2 x) → τ.[s1] = τ.[s2].
+Proof.
+  intros Htyped; revert s1 s2.
+  assert (∀ {A} `{Ids A} `{Rename A}
+            (s1 s2 : nat → A) x, (x ≠ 0 → s1 (pred x) = s2 (pred x)) → up s1 x = up s2 x).
+  { intros A H1 H2. rewrite /up=> s1 s2 [|x] //=; auto with f_equal omega. }
+  induction Htyped => s1 s2 Hs; f_equal/=; eauto using lookup_lt_Some with omega.
+Qed.
+
+Fixpoint iter (n : nat) `(f : A → A) :=
+  match n with
+  | O => λ x, x
+  | S n' => λ x, f (iter n' f x)
+  end.
+
+Lemma iter_S (n : nat) `(f : A → A) (x : A) : iter (S n) f x = iter n f (f x).
+Proof.
+  induction n; cbn; trivial.
+  rewrite -IHn; trivial.
+Qed.
+  
+Lemma iter_upren (m n x : nat) : iter m upren (+n) x = if lt_dec x m then x else n + x.
+Proof.
+  revert n x; induction m; cbn; auto with omega.
+  intros n x; destruct x; cbn; trivial.
+  rewrite IHm; repeat destruct lt_dec; auto with omega.
+Qed.
+
+Lemma closed_type_S_ren1:
+  ∀ (τ : type) (n m : nat) (k : nat) (Hle : m ≤ k),
+    (closed_type (n + k) τ.[ren ((iter m upren) (+n))] → closed_type k τ).
+Proof.
+  induction τ; intros n m k Hle H; inversion H; subst; constructor; eauto 2 with omega.
+  - eapply (IHτ n (S m)); asimpl in *; auto with omega.
+  - rewrite iter_upren in H1; destruct lt_dec; omega.
+  - eapply (IHτ n (S m)); asimpl in *; auto with omega.
+Qed.
+
+Lemma closed_type_S_ren2:
+  ∀ (τ : type) (n m : nat) (k : nat) (Hle : m ≤ k),
+    (closed_type k τ → closed_type (n + k) τ.[ren ((iter m upren) (+n))]).
+Proof.
+  induction τ; intros n m k Hle H; inversion H; subst; constructor; eauto 2 with omega.
+  - replace (up (ren (iter m upren (+n)))) with
+    (ren (iter (S m) upren (+n))) by (asimpl; trivial).
+    replace (S (n + k)) with (n + (S k)) by omega. auto with omega.
+  - rewrite iter_upren; destruct lt_dec; omega.
+  - replace (up (ren (iter m upren (+n)))) with
+    (ren (iter (S m) upren (+n))) by (asimpl; trivial).
+    replace (S (n + k)) with (n + (S k)) by omega. auto with omega.
+Qed.
+
+Lemma closed_type_pred_ren1:
+  ∀ (τ : type) (n m : nat) (k : nat),
+    (closed_type k τ.[ren ((iter m upren) (iter n pred))] → closed_type (n + k) τ).
+Proof.
+  induction τ; intros n m k H; inversion H; subst; constructor; eauto 2 with omega.
+  - replace (S (n + k)) with (n + (S k)) by omega.
+    apply IHτ with (S m).
+    replace (up (ren (iter m upren (iter n pred)))) with
+    (ren (iter (S m) upren (iter n pred))) in H1 by (asimpl; trivial); trivial.
+  - admit.
+  - replace (S (n + k)) with (n + (S k)) by omega.
+    apply IHτ with (S m).
+    replace (up (ren (iter m upren (iter n pred)))) with
+    (ren (iter (S m) upren (iter n pred))) in H1 by (asimpl; trivial); trivial.
+Admitted.
+
+Lemma closed_type_pred_ren2:
+  ∀ (τ : type) (n m : nat) (k : nat),
+    closed_type (n + k) τ → closed_type k τ.[ren ((iter m upren) (iter n pred))].
+Proof.
+  induction τ; intros n m k H; inversion H; subst; constructor; eauto 2 with omega.
+  - replace (up (ren (iter m upren (iter n pred)))) with
+    (ren (iter (S m) upren (iter n pred))) by (asimpl; trivial); trivial.
+    eapply (IHτ n (S m)); asimpl in *; auto with omega.
+  - admit.
+  - replace (up (ren (iter m upren (iter n pred)))) with
+    (ren (iter (S m) upren (iter n pred))) by (asimpl; trivial); trivial.
+    eapply (IHτ n (S m)); asimpl in *; auto with omega.
+Admitted.
+
+Lemma closed_ctx_map_S:
+  ∀ (k : nat) (Γ : list type), closed_ctx (S k) (map (λ t : type, t.[ren (+1)]) Γ) → closed_ctx k Γ.
+Proof.
+  intros k Γ H.
+  induction Γ; constructor; inversion H; subst.
+  eapply closed_type_S_ren1 with 1 0; cbn; auto with omega.
+  apply IHΓ; trivial.
+Qed.
+
+Lemma typed_closed_type (k : nat) (Γ : list type) (e : expr) (τ : type) :
+  typed k Γ e τ → closed_ctx k Γ ∧ closed_type k τ.
+Proof.
+  intros H; induction H; intuition.
+  - eapply closed_ctx_closed_type; eauto.
+  - eauto 3.
+  - eauto 3.
+  - inversion H0; trivial.
+  - inversion H0; auto.
+  - inversion H2; trivial.
+  - apply closed_ctx_map_S; trivial.
+  - inversion H2; subst.
+
+    Lemma closed_type_subst:
+      ∀ (k : nat) (τ : {bind type}) (τ' : type),
+        closed_type k τ' → closed_type (S k) τ → closed_type k τ.[τ' .: ren pred].
+    Proof.
+      intros k τ; revert k.
+      induction τ; intros k τ' H1 H2; try constructor; inversion H2; subst; auto.
+      replace (τ.[up (τ' .: ren Init.Nat.pred)]) with
+      (τ.[up (τ' .: ren Init.Nat.pred)])
+
+      
+      apply (closed_type_pred_ren2).
+
+      asimpl in *.
+      replace (ids 0 .: τ'.[ren (+1)] .: ren (Init.Nat.pred >>> (+1))) with
+      (ids 0 .: τ'.[ren (+1)] .: ids 1 .: ren S).
+      Focus 2.
+      extensionality x.
+      do 3 try destruct x; cbn; trivial.
+      
+      
+      
+      
+      apply closed_type_S_ren with 0 1; auto with omega.
+      asimpl in *.
+      
+
+      
+      
+  - apply closed_ctx_map_S; trivial.
+  - inversion H1; subst.
+
+
+
+
+Local Hint Extern 1 =>
+match goal with [H : context [length (map _ _)] |- _] => rewrite map_length in H end
+: typed_subst_invariant.
+
+Lemma typed_subst_invariant k Γ e τ s1 s2 :
+  typed k Γ e τ → (∀ x, x < length Γ → s1 x = s2 x) → e.[s1] = e.[s2].
+Proof.
+  intros Htyped; revert s1 s2.
+  assert (∀ {A} `{Ids A} `{Rename A}
+            (s1 s2 : nat → A) x, (x ≠ 0 → s1 (pred x) = s2 (pred x)) → up s1 x = up s2 x).
+  { intros A H1 H2. rewrite /up=> s1 s2 [|x] //=; auto with f_equal omega. }
+  induction Htyped => s1 s2 Hs; f_equal/=; eauto using lookup_lt_Some with omega typed_subst_invariant.
+  sadfas dfasdfas.
+Qed.
+
+    
 Import uPred.
 
 Lemma Forall2_inside_forall {A B C} (x : C) (P : C → A → B → Prop) (l : list A) (l' : list B) :
@@ -964,20 +1130,6 @@ Section typed_interp.
     
   Definition env_subst (vs : list val) (x : var) : expr :=
     from_option (Var x) (of_val <$> vs !! x).
-
-  Local Hint Extern 1 =>
-  match goal with [H : context [length (map _ _)] |- _] => rewrite map_length in H end
-  : typed_subst_invariant.
-  
-  Lemma typed_subst_invariant k Γ e τ s1 s2 :
-    typed k Γ e τ → (∀ x, x < length Γ → s1 x = s2 x) → e.[s1] = e.[s2].
-  Proof.
-    intros Htyped; revert s1 s2.
-    assert (∀ {A} `{Ids A} `{Rename A}
-              (s1 s2 : nat → A) x, (x ≠ 0 → s1 (pred x) = s2 (pred x)) → up s1 x = up s2 x).
-    { intros A H1 H2. rewrite /up=> s1 s2 [|x] //=; auto with f_equal omega. }
-    induction Htyped => s1 s2 Hs; f_equal/=; eauto using lookup_lt_Some with omega typed_subst_invariant.
-  Qed.
   
   Lemma typed_subst_head_simpl k Δ τ e w ws :
     typed k Δ e τ -> length Δ = S (length ws) →
@@ -989,24 +1141,6 @@ Section typed_interp.
     destruct (lookup_lt_is_Some_2 ws x) as [v' Hv]; first omega; simpl.
       by rewrite Hv.
   Qed.
-
-  Local Tactic Notation "smart_wp_bind" uconstr(ctx) uconstr(t) ident(v) :=
-    rewrite -(@wp_bind _ _ _ [ctx]) /= -wp_impl_l; apply and_intro; eauto with itauto;
-    apply (@always_intro _ _ _ t), forall_intro=> v /=; apply impl_intro_l.
-
-  Local Tactic Notation "smart_wp_bind" uconstr(ctx) ident(v) :=
-    rewrite -(@wp_bind _ _ _ [ctx]) /= -wp_mono; eauto; intros v; cbn.
-
-
-  Local Hint Extern 1 ((_ ∧ _) ⊑ _)%I => rewrite and_elim_r : itauto.
-  Local Hint Extern 1 ((_ ∧ _) ⊑ _)%I => rewrite and_elim_l : itauto.
-  Local Hint Extern 1 (_ ⊑ (_ ∧ _))%I => repeat eapply and_intro : itauto.
-  Local Hint Extern 1 (_ ⊑ ▷ _)%I => rewrite -later_intro : itauto.
-  Local Hint Extern 1 (_ ⊑ ∃ _, _)%I => rewrite -exist_intro : itauto.
-  Local Hint Extern 1 (_ ⊑ (_ ∨ _))%I => rewrite -or_intro_l : itauto.
-  Local Hint Extern 1 (_ ⊑ (_ ∨ _))%I => rewrite -or_intro_r : itauto.
-
-  Local Ltac value_case := rewrite -wp_value/= ?to_of_val //.
 
   Class VlistAlwaysStable {k} (Δ : Vlist (leibniz_val -n> iProp lang Σ) k) :=
     vlistalwaysstable : Forall (λ f, (∀ v : val, AlwaysStable ((cofe_mor_car _ _ f) v))) (` Δ).
@@ -1037,9 +1171,35 @@ Section typed_interp.
            (Hctx : closed_ctx k Γ)
            {HΔ : VlistAlwaysStable Δ}
     : AlwaysStable (Π∧ zip_with (λ τ v, interp k (` τ) (proj2_sig τ) Δ v) (closed_ctx_list _ Γ Hctx) vs)%I.
-  Proof.
-    typeclasses eauto.
-  Qed.
+  Proof. typeclasses eauto. Qed.
+
+  Ltac ipropsimpl :=
+    repeat
+      match goal with
+      | [|- (_ ⊑ (_ ∧ _))%I] => eapply and_intro
+      | [|- (▷ _ ⊑ ▷ _)%I] => apply later_mono
+      | [|- (_ ⊑ ∃ _, _)%I] => rewrite -exist_intro
+      | [|- ((∃ _, _) ⊑ _)%I] => let v := fresh "v" in rewrite exist_elim; [|intros v]
+      end.
+
+  Local Hint Extern 1 => progress ipropsimpl.
+
+  Local Tactic Notation "smart_wp_bind" uconstr(ctx) uconstr(t) ident(v) :=
+    rewrite -(@wp_bind _ _ _ [ctx]) /= -wp_impl_l; apply and_intro; [
+    apply (@always_intro _ _ _ t), forall_intro=> v /=; apply impl_intro_l| eauto with itauto].
+
+  Local Tactic Notation "smart_wp_bind" uconstr(ctx) ident(v) :=
+    rewrite -(@wp_bind _ _ _ [ctx]) /= -wp_mono; eauto; intros v; cbn.
+
+  Create HintDb itauto.
+
+  Local Hint Extern 3 ((_ ∧ _) ⊑ _)%I => rewrite and_elim_r : itauto.
+  Local Hint Extern 3 ((_ ∧ _) ⊑ _)%I => rewrite and_elim_l : itauto.
+  Local Hint Extern 3 (_ ⊑ (_ ∨ _))%I => rewrite -or_intro_l : itauto.
+  Local Hint Extern 3 (_ ⊑ (_ ∨ _))%I => rewrite -or_intro_r : itauto.
+  Local Hint Extern 2 (_ ⊑ ▷ _)%I => etransitivity; [|rewrite -later_intro] : itauto.
+  
+  Local Ltac value_case := rewrite -wp_value/= ?to_of_val //.
 
   Lemma typed_interp k Δ Γ vs e τ
         (Htyped : typed k Γ e τ)
@@ -1063,33 +1223,33 @@ Section typed_interp.
       apply interp_closed_irrel.
     - (* unit *) value_case.
     - (* pair *)
-      smart_wp_bind (PairLCtx e2.[env_subst vs]) _ v.
+      smart_wp_bind (PairLCtx e2.[env_subst vs]) _ v; eauto.
       (* weird!: and_alwaysstable is an instance but is not resolved! *)
       smart_wp_bind (PairRCtx v) (and_always_stable _ _ _ _) v'.
-      value_case.
-      
-      
-  - (* fst *)
-    smart_wp_bind (FstCtx) v.
-    rewrite exist_elim; eauto; intros v1. rewrite exist_elim; eauto; intros v2.
-    apply const_elim_l; intros H; rewrite H.
-    rewrite -wp_fst; eauto using to_of_val, and_elim_l.
-  - (* snd *)
-    smart_wp_bind SndCtx v.
-    rewrite exist_elim; eauto; intros v1. rewrite exist_elim; eauto; intros v2.
-    apply const_elim_l; intros H; rewrite H.
-    rewrite -wp_snd; eauto using to_of_val, and_elim_r.
-  - (* injl *) smart_wp_bind InjLCtx v; value_case; eauto 7 with itauto.
-  - (* injr *) smart_wp_bind InjRCtx v; value_case; eauto 7 with itauto.
-  - (* case *)
-    smart_wp_bind (CaseCtx _ _) _ v.
-    rewrite (later_intro (Π∧ zip_with interp Γ vs)).
+      value_case; eauto 10 with itauto.
+    - (* fst *)
+      smart_wp_bind (FstCtx) v. ipropsimpl; eauto.
+      apply const_elim_l; intros H; rewrite H.
+      rewrite -wp_fst; eauto using to_of_val, and_elim_l.
+      rewrite and_elim_l; rewrite interp_closed_irrel; eauto.
+    - (* snd *)
+      smart_wp_bind SndCtx v. ipropsimpl; eauto.
+      apply const_elim_l; intros H; rewrite H.
+      rewrite -wp_snd; eauto using to_of_val, and_elim_l.
+      rewrite and_elim_r; rewrite interp_closed_irrel; eauto.
+    - (* injl *) smart_wp_bind InjLCtx v; value_case; eauto 7 with itauto.
+    - (* injr *) smart_wp_bind InjRCtx v; value_case; eauto 7 with itauto.
+    - (* case *)
+      smart_wp_bind (CaseCtx _ _) _ v. cbn.
+      rewrite (later_intro (Π∧ zip_with
+           (λ (τ : {τ : type | closed_type k τ}) (v0 : leibniz_val),
+            ((interp k (` τ) (proj2_sig τ)) Δ) v0) (closed_ctx_list k Γ Hctx) vs)).
     rewrite or_elim; [apply impl_elim_l| |];
     rewrite exist_elim; eauto; [intros v1| intros v2];
     apply const_elim_l; intros H; rewrite H;
     rewrite -impl_intro_r // -later_and later_mono; eauto;
-    [rewrite -wp_case_inl | rewrite -wp_case_inr]; eauto using to_of_val;
-    asimpl; [specialize (IHHtyped2 (v1::vs)) | specialize (IHHtyped3 (v2::vs))];
+    [rewrite -wp_case_inl | rewrite -wp_case_inr]; eauto using to_of_val.
+    asimpl. specialize (IHHtyped2 Δ HC (v1::vs)). | specialize (IHHtyped3 (v2::vs))];
     erewrite <- ?typed_subst_head_simpl in * by (cbn; eauto);
     [rewrite -IHHtyped2 | rewrite -IHHtyped3]; cbn; auto.
   - (* lam *)
